backup changes

TeryGrad/Ops/UShape.lean
@@ -1,22 +1,39 @@
 import TeryGrad.Shape.ShapeTracker
 import TeryGrad.Ops.U
+import TeryGrad.Helpers
 
 namespace UOp
 
-def st (self : UOp) : Option ShapeTracker := Id.run do
+partial def listlize (self:UOp) : ListTree (Int × Option (ConstLike ⊕ ShapeTracker) × Option DType) :=
+  ListTree.mk (self.op.value, self.arg, self.dtype) (self.src.map (fun x => x.listlize))
+
+instance : Inhabited UOp := sorry
+instance : BEq ShapeTracker := sorry
+
+partial def st (self : UOp) : Option ShapeTracker
+:= Id.run do
     if self.op == Ops.VIEW then
       match self.arg with
-      | some x => match x with
-        | Sum.inl _ => pure ()
-        | Sum.inr x' => return x'
-      | none => pure ()
-    return none
-    -- -- buffer ops can have a non contiguous shapetracker
-    -- if self.op in GroupOp.Buffer and len(src_sts:=[unwrap(x.st) for x in self.src if x.op is Ops.VIEW]) != 0: return src_sts[0]
-    -- if len(src_sts:=[x.st for x in self.src if x.st is not None]) == 0: return None
+      | some (Sum.inr x) => return x
+      | _ => pure ()
+    -- buffer ops can have a non contiguous shapetracker
+    if GroupOp.Buffer.contains self.op then
+      let src_sts : List ShapeTracker := (self.src.filter (fun x => x.op == Ops.VIEW)).filterMap (fun x => unwrap x.st)
+      if src_sts.length != 0 then return src_sts.get! 0
+    -- get all non none srcs
+    let src_sts : List ShapeTracker := self.src.filterMap (fun x => x.st)
+    if src_sts.length == 0 then return none
     -- assert all_same([x.shape for x in src_sts]), f"UOp parents must have the same shape {self} {[x.shape for x in src_sts]}"
-    -- # all other ops have a contiguous shapetracker
-    -- return ShapeTracker.from_shape(src_sts[0].reduce(self.axis_arg) if self.op in (Ops.REDUCE_AXIS, Ops.WMMA) else src_sts[0].shape)
+    -- buffer ops can have a non contiguous shapetracker
+    return ShapeTracker.from_shape (if [Ops.REDUCE_AXIS, Ops.WMMA].contains self.op then (src_sts.get! 0).reduce self.axis_arg else (src_sts.get! 0).shape)
+def shape (self : UOp) : List SInt := (unwrap self.st).shape
+partial def full_shape (self : UOp) : List SInt :=
+  if self.op == Ops.VIEW then self.shape else
+    self.src.filter (fun x => x.st.isSome) |>.map (smax ∘ full_shape)
+def size (self : UOp) : Int :=
+  if self.op == Ops.BUFFER then self.arg[1][1] else (unwrap self.st).size
 
+
+  -- tuple(smax(x) for x in zip(*[x.full_shape for x in self.src if x.has_st]))
 end UOp
 -- UOp methods that depend on ShapeTracker
