TeryGrad/Minimal/mwe.lean
@@ -1,0 +1,14 @@
+example (A B : Array Nat) : A = B := by
+    ext i h1 h2
+
+
+/- case h₁
+    A B : Array Nat
+    ⊢ A.size = B.size
+case h₂
+    A B : Array Nat
+    i✝ : Nat
+    hi₁✝ : i✝ < A.size
+    hi₂✝ : i✝ < B.size
+    ⊢ A[i✝] = B[i✝]
+-/
