TeryGrad/Ops/U.lean
@@ -1,11 +1,10 @@
 import TeryGrad.Ops.basic
 import Std.Data.HashMap.Basic
 import TeryGrad.FromPython
-
 -- method definitions for UOp and UPat
 
 namespace UOp
-def UOp.default (op : Ops) := UOp.mk op DType.void [] none
+-- def UOp.default (op : Ops) := UOp.mk op DType.void [] none
 
 def alu : UOp → Ops → List Uop → UOp := sorry
 -- out_dtype = (self, *src)[-1].dtype
@@ -15,9 +14,7 @@ def alu : UOp → Ops → List Uop → UOp := sorry
 def const_like : UOp → ConstLike → UOp := sorry
 instance : MathTrait UOp := {
   alu := alu, const_like := const_like,
-  dtype := fun x =>
-    match x with
-    | UOp.mk _ dtype _ _ => dtype
+  dtype := fun x => x.dtype
 }
 
 -- instance : ToString UOp :=
@@ -41,13 +38,12 @@ inductive ListTree (α : Type u)
 
 instance {α : Type u} [Inhabited α] : Inhabited (ListTree α) := ⟨ListTree.mk Inhabited.default []⟩
 
-partial def listlize (self:UOp) : ListTree (Int × Option (ConstLike ⊕ ShapeTracker) × Option DType) :=
-  ListTree.mk (self.op.value, self.arg, self.dtype) (self.src.map listlize)
-
 instance : BEq Ops := sorry
 def has_st (self : UOp) : Bool := [Ops.DEFINE_LOCAL, Ops.DEFINE_GLOBAL, Ops.BUFFER, Ops.CONST, Ops.DEFINE_VAR].contains self.op
 
 instance : Coe UOp Bool := sorry
+
+def axis_arg (self : UOp) : List Int := sorry
 
 #check Std.HashMap
 #check String.hash
