README.md
@@ -8,5 +8,13 @@ better overall type safety:
 - The behavior of the SimpleMathTrait type is much more explicit
 potential for formally verified correctness.
 - We can require that new function definitions must prove that they satisfy the preconditions of stochastic gradient descent via a Sigma type.
+- Shape matching can be enforced as a type constraint. Meanning that shape errors show up as type errors. This has the additional benefit of bypassing the need for a dedicated shape inference engine. Since we can use lean's type inference engine to do the work. For example in tinygrad you would do (-1, 2, 3) but in terygrad you would do [_, 2, 3] (using the hole command to indicate that lean should try to infer the value of _ at elaboration/compile time)
 
 Just as how TinyGrad's size allows it to implement accelerators quickly, TeryGrad's verification abilities allow new models to implmeented quickly with guaranteed convergence properties
+
+
+# resources
+
+https://github.com/mesozoic-egg/tinygrad-notes/
+
+see TeryGrad/Minimal for implmentation of a simplified version of TinyGrad (so you can see how all the moving parts come together)
